Working on time bound fix

src/polyfix.lean
@@ -1,23 +1,46 @@
 import polycodable
 
 variables {α β : Type*}
-def fix_bounded_iter (f : α → β ⊕ α) : ℕ → α → option β
+
+def fix_bounded_while (f : α → β ⊕ α) (P : α → Prop) [decidable_pred P] : ℕ → α → option β
 | 0 x := none
-| (n + 1) x := match f x with
+| (n + 1) x := if P x then match f x with
   | (sum.inl y) := some y
-  | (sum.inr x') := fix_bounded_iter n x'
+  | (sum.inr x') := fix_bounded_while n x'
+end else none
+
+def fix_bounded_terminates (f : α → β ⊕ α) (P : α → Prop) [decidable_pred P] (i : ℕ) (x : α) : Prop :=
+(fix_bounded_while f P i x).is_some
+
+lemma not_fix_bounded_terminates_zero (f : α → β ⊕ α) (P : α → Prop) [decidable_pred P] (x : α) :
+  ¬fix_bounded_terminates f P 0 x := by trivial
+
+lemma fix_bounded_terminates_iff (f : α → β ⊕ α) (P : α → Prop) [decidable_pred P] (i : ℕ) (x : α) :
+  (fix_bounded_terminates f P (i+1) x) ↔ P x ∧ (∀ x', f x = sum.inr x' → fix_bounded_terminates f P i x') :=
+begin
+  simp only [fix_bounded_terminates, fix_bounded_while],
+  split_ifs with H, swap, { simp [H], },
+  cases hf : f x; simp [fix_bounded_while, H],
 end
 
-lemma fix_eq_fix_bounded {f : α → β ⊕ α} {x : α} {y : β} {i : ℕ}
-  (h : y ∈ fix_bounded_iter f i x) : y ∈ pfun.fix (f : α →. β ⊕ α) x :=
+lemma fix_eq_fix_bounded {f : α → β ⊕ α} {P : α → Prop} [decidable_pred P] {x : α} {y : β} {i : ℕ}
+  (h : y ∈ fix_bounded_while f P i x) : y ∈ pfun.fix (f : α →. β ⊕ α) x :=
 begin
   induction i with i ih generalizing x,
-  { simp [fix_bounded_iter] at h, contradiction, },
+  { simp [fix_bounded_while] at h, contradiction, },
+  simp only [fix_bounded_while] at h, split_ifs at h with _, swap, { trivial, },
   cases H : f x with vl vr,
-  { apply pfun.fix_stop, simp [fix_bounded_iter, H] at h ⊢, exact h.symm, },
-  specialize ih (by simpa [fix_bounded_iter, H, ← option.mem_def] using h),
+  { apply pfun.fix_stop, simp [fix_bounded_while, H] at h ⊢, exact h.symm, },
+  specialize ih (by simpa [fix_bounded_while, H, ← option.mem_def] using h),
   rw [@comm _ (=), ← part.mem_some_iff, ← pfun.coe_val] at H,
   rwa pfun.fix_fwd _ _ H,
+end
+
+lemma dom_of_fix_bounded_terminates {f : α → β ⊕ α} {P : α → Prop} [decidable_pred P] {x : α} {i : ℕ}
+  (h : fix_bounded_terminates f P i x) : (pfun.fix (f : α →. β ⊕ α) x).dom :=
+begin
+  rw [fix_bounded_terminates, option.is_some_iff_exists] at h, rcases h with ⟨y, hy⟩,
+  rw part.dom_iff_mem, use [y, fix_eq_fix_bounded hy],
 end
 
 section poly
@@ -44,16 +67,79 @@ lemma code_fix_eq_pfun_fix' {f : α → β ⊕ α} {c : code} (hfc : ∀ x, c.ev
   c.fix.eval (encode x) = (pfun.fix (f : α →. β ⊕ α) x).map encode :=
 by { apply code_fix_eq_pfun_fix, simp [hfc], }
 
+lemma eval_fix_fun_dom_eq_dom {c : code} : pfun.dom (eval_fix_fun c) = c.eval.dom :=
+by simp [pfun.dom]
+
 abbreviation encode_sizeof (x : α) := (encode x).sizeof
 
-lemma polytime_fix_bounded (p : polynomial ℕ) (f : α → β ⊕ α) (g : α → β)
-  (hf : ∀ x, g x ∈ fix_bounded_iter f (p.eval (encode_sizeof x)) x) 
-  (bg : ∃ C : ℕ, ∀ x, encode_sizeof (f x) ≤ (encode_sizeof x) + C) : polytime_fun f → polytime_fun g :=
+section time_bound_fix_lemma
+
+lemma time_bound_of_fix_bounded_terminates {c : code} {x : ptree}
+  (hc : c.eval.dom = set.univ) {T J : ℕ}
+  (ht : fix_bounded_terminates (pfun.to_fun (eval_fix_fun c) (by rwa eval_fix_fun_dom_eq_dom))
+    (λ x', (c.time.to_fun (by rwa time_dom_eq_eval_dom) x') ≤ T) J x) :
+  ∃ t ∈ c.fix.time x, t ≤ J * T + 1 :=
+begin
+  induction J with j ih generalizing x,
+  { exfalso, exact not_fix_bounded_terminates_zero _ _ _ ht, },
+  have : (c.fix.time x).dom,
+  { rw [time_dom_iff_eval_dom, code_fix_eval], simpa using dom_of_fix_bounded_terminates ht,},
+  rw part.dom_iff_mem at this, cases this with t H, use [t, H],
+  rw fix_bounded_terminates_iff at ht, cases ht with ht₁ ht₂,
+  cases fv : pfun.to_fun (eval_fix_fun c) (by rwa eval_fix_fun_dom_eq_dom) x with y x',
+  { clear ih ht₂, simp [pfun.to_fun, eval_fix_fun] at fv, simp [pfun.to_fun, code_fix_time] at H,
+    rcases H with ⟨t', ht', rfl⟩,
+    cases fv with fv₁ fv₂,
+    simp only [add_le_add_iff_right],
+    have : ∃ t'', sum.inl t'' ∈ time_fix_fun c (x, 0),
+    { use (c.time.to_fun (by rwa time_dom_eq_eval_dom) x), 
+      simp [time_fix_fun], } }
+end
+
+
+private def c_invariant (c : code) (hc : c.eval.dom = set.univ) (v : ptree) (T M : ℕ) : Prop :=
+  fix_bounded_terminates
+    (pfun.to_fun (eval_fix_fun c) (by rwa eval_fix_fun_dom_eq_dom))
+    (λ x, x.sizeof ≤ M) 
+    T v
+
+lemma time_bound_fix {c : code} {b₁ b₂ m : ℕ → ℕ} (hb₁ : time_bound c b₁)
+  (hb₂ : ∀ x : ptree, c_invariant c (eval_dom_of_time_bound hb₁) x (b₂ x.sizeof) (m x.sizeof)) : time_bound c.fix (λ t, (b₁ $ m t) * (b₂ t) + 1) :=
+begin
+  intros n v hnv,
+  have : (c.fix.time v).dom,
+  { rw [time_dom_iff_eval_dom, code_fix_eval], simpa using dom_of_fix_bounded_terminates (hb₂ v), },
+  rw part.dom_iff_mem at this, rcases this with ⟨t, ht⟩, use [t, ht],
+  simp only [code_fix_time, part.mem_map_iff, part.map_eq_map] at ht, rcases ht with ⟨t', ht, rfl⟩, dsimp only,
+  simp only [add_le_add_iff_right], -- Invariant: fix_bounded_terminates (pfun.to_fun ...) ... (b₂ x.sizeof) - t
+  refine pfun.fix_induction_invariant (λ vt : ptree × ℕ, c_invariant c (eval_dom_of_time_bound hb₁) vt.1 ((b₂ v.sizeof) - vt.2) (m v.sizeof)) ht _ _ _,
+  { simpa using hb₂ _, },
+  { rintros ⟨x₁, t₁⟩ ⟨x₂, t₂⟩ hx₁ hx₂, dsimp only,
+    simp [c_invariant], }
+end
+
+end time_bound_fix_lemma
+
+#exit
+
+lemma polytime_fix_bounded (p q : polynomial ℕ) (f : α → β ⊕ α) (g : α → β)
+  (hf : ∀ x, g x ∈ fix_bounded_while f (λ x' : α, encode_sizeof x' ≤ q.eval (encode_sizeof x)) (p.eval (encode_sizeof x)) x) :
+  polytime_fun f → polytime_fun g :=
 begin
   rintro ⟨c, pc, s⟩,
   use code.fix c, split, swap,
   { intro x, simp only [part.eq_some_iff], rw code_fix_eq_pfun_fix' s, simpa using fix_eq_fix_bounded (hf x), },
-  
+  -- Max output value: q(x), max time per step: pc(q(x)), max time: p(x)pc(q(x))
 end
+
+-- lemma polytime_fix_bounded (p : polynomial ℕ) (f : α → β ⊕ α) (g : α → β)
+--   (hf : ∀ x, g x ∈ fix_bounded_iter f (p.eval (encode_sizeof x)) x) 
+--   (bg : ∃ C : ℕ, ∀ x, encode_sizeof (f x) ≤ (encode_sizeof x) + C) : polytime_fun f → polytime_fun g :=
+-- begin
+--   rintro ⟨c, pc, s⟩,
+--   use code.fix c, split, swap,
+--   { intro x, simp only [part.eq_some_iff], rw code_fix_eq_pfun_fix' s, simpa using fix_eq_fix_bounded (hf x), },
+  
+-- end
 
 end poly
